src/LLBC.v
@@ -300,11 +300,11 @@ Variant store (p : place) : LLBC_val * LLBC_state -> LLBC_state -> Prop :=
 
 (* When introducing non-terminating features (loops or recursivity), the signature of the relation
    is going to be:
-   LLBC_state -> statement -> nat -> Option (statement_result * LLBC_state) -> Prop
+   LLBC_state -> statement -> nat -> Option (flow_token * LLBC_state) -> Prop
 *)
 Reserved Notation "S  |-{stmt}  stmt  =>  r , S'" (at level 50).
 
-Inductive eval_stmt : statement -> statement_result -> LLBC_state -> LLBC_state -> Prop :=
+Inductive eval_stmt : statement -> flow_token -> LLBC_state -> LLBC_state -> Prop :=
   | Eval_nop S : S |-{stmt} Nop => rUnit, S
   | Eval_panic S : S |-{stmt} Panic => rPanic, S
   | Eval_seq_unit S0 S1 S2 stmt_l stmt_r r (eval_stmt_l : S0 |-{stmt} stmt_l => rUnit, S1)
